\section{Derivation}

From the problem statement we have the following system of PDEs.
\begin{subequations} \label{eq:system}
\begin{align}
    u_t &= D_u u_{xx} + u \left( 1 - u - \frac{av}{1+\lambda u} \right) \label{eq:prey} \\
    v_t &= D_v v_{xx} - v \left( \frac{1}{ab} - \frac{au}{b(1+\lambda u)} \right) \label{eq:pred} \\
    \notag\\
        &  a \leq x \leq b, \quad 0 \leq t \leq T \notag
\end{align}
\end{subequations}

We use the following finite difference approximations, derived from the Taylor
series expansion, in place of the $u_t$, $u_{xx}$, $v_t$, and $v_{xx}$ in
equations \eqref{eq:system}. The spacial and temporal domains are descretized
using $N$ and $M$ points respectively and $h$ and $k$ are the related step
lengths.
\begin{subequations} \label{eq:taylor}
\begin{align}
    u_t &= \frac{u(x,t+k)-u(x,t)}{k} - \frac{k}{2} u_{tt}(x,\tau) \label{eq:u_t}
    \\
    v_t &= \frac{v(x,t+k)-v(x,t)}{k} - \frac{k}{2} v_{tt}(x,\sigma) \label{eq:v_t}
    \\
    u_{xx} &= \frac{u(x-h,t)-2u(x,t)+u(x+h,t)}{h^2} -
        \frac{h^2}{12} u_{xxxx}(\xi,t) \label{eq:u_xx}
    \\
    v_{xx} &= \frac{v(x-h,t)-2v(x,t)+v(x+h,t)}{h^2} -
        \frac{h^2}{12} v_{xxxx}(\epsilon,t) \label{eq:v_xx}
\end{align}
\end{subequations}

Let $n = 1 \dots N$ and $m = 1 \dots M$. Discard the truncation terms from
equations \eqref{eq:taylor} and let $U_n^m$ and $V_n^m$ approximate the true
solutions $u(x_n,t_m)$ and $v(x_n,t_m)$. The initial $u$ and $v$ in the source
terms from \eqref{eq:system} are replaced with the central differences:
\begin{subequations} \label{eq:source_term_approx}
\begin{align}
    u &= \frac{U_n^{m+1} + U_n^m}{2} \\
    v &= \frac{V_n^{m+1} + V_n^m}{2}
\end{align}
\end{subequations}

We can then replace equations \eqref{eq:system} with the following system of
equations.
\begin{subequations} \label{eq:approx_sys}
\begin{align}
    \frac{U_{n}^{m+1} - U_{n}^{m}}{k} &=
        \frac{D_u}{2} \left\{
           \left[ \frac{U_{n-1}^{m+1}-2U_{n}^{m+1}+U_{n+1}^{m+1}}{h^2} \right] +
            \left[ \frac{U_{n-1}^{m}-2U_{n}^{m}+U_{n+1}^{m}}{h^2} \right]
        \right\} \notag\\
        &+ \left[ \frac{U_n^{m+1} + U_n^m}{2} \right]
           \left[ 1 - U_n^m - \frac{a V_n^m}{1 + \lambda U_n^m} \right]
           \label{eq:approx_prey}
        \\ \notag
        \\
    \frac{V_{n}^{m+1} - V_{n}^{m}}{k} &=
        \frac{D_v}{2} \left\{
           \left[ \frac{V_{n-1}^{m+1}-2V_{n}^{m+1}+V_{n+1}^{m+1}}{h^2} \right] +
           \left[ \frac{V_{n-1}^{m}-2V_{n}^{m}+V_{n+1}^{m}}{h^2} \right]
        \right\} \notag\\
        &- \left[ \frac{V_n^{m+1} + V_n^m}{2} \right]
           \left[ \frac{1}{ab} - \frac{a U_n^m}{b ( 1 + \lambda U_n^m )} \right]
           \label{eq:approx_pred}
\end{align}
\end{subequations}

Multiplying equations \eqref{eq:approx_sys} throughout by $2k$ and rearranging
the terms such that all the $U^{m+1}$ and $V^{m+1}$ terms are taken to the LHS
yields the following with $r = D_u k / h^2$ and $s = D_v k / h^2$:
\begin{subequations} \label{eq:rearranged_approx_sys}
\begin{align}
    -r U_{n-1}^{m+1} +
    \left(
        2 + 2r - k + k U_n^m + \frac{a k V_n^m}{1 + \lambda U_n^m}
    \right)
    U_n^{m+1} - r U_{n+1}^{m+1} \notag
    \\
    = r U_{n-1}^m +
    \left(
        2 - 2r + k - k U_n^m - \frac{a k V_n^m}{1 + \lambda U_n^m}
    \right)
    U_n^m + r U_{n+1}^m
    \\
    \notag
    \\
    -s V_{n-1}^{m+1} +
    \left(
        2 + 2s + \frac{k}{ab} - \frac{a k U_n^m}{b ( 1 + \lambda U_n^m )}
    \right)
    V_n^{m+1} - s V_{n+1}^{m+1} \notag
    \\
    = s V_{n-1}^m +
    \left(
        2 - 2s - \frac{k}{ab} + \frac{a k U_n^m}{b ( 1 + \lambda U_n^m )}
    \right)
    V_n^m + s V_{n+1}^m
\end{align}
\end{subequations}

We now investigate the boundary conditions. When $n=1$ we have may use the
central difference formula for the first derivatives as follows:
\begin{subequations}
\begin{align}
    U_x(a,t) &= 0 = \frac{{U_2} - U_{0}}{2h} \\
    V_x(a,t) &= 0 = \frac{{V_2} - V_{0}}{2h}
\end{align}
\end{subequations}

Since the derivatives at the boundaries are given as 0 this implies that:
\begin{subequations} \label{eq:left_end_points}
\begin{align}
    U_{2} &= U_{0} \\
    V_{2} &= V_{0}
\end{align}
\end{subequations}

The same argument follows for the right endpoint where $n=N$ and we have:
\begin{subequations}
\begin{align}
    U_x(b,t) &= 0 = \frac{{U_{N+1}} - U_{N-1}}{2h} \\
    V_x(b,t) &= 0 = \frac{{V_{N+1}} - V_{N-1}}{2h}
\end{align}
\end{subequations}
hence we find that
\begin{subequations} \label{eq:right_end_points}
\begin{align}
    U_{N+1} &= U_{N-1} \\
    V_{N+1} &= V_{N-1}
\end{align}
\end{subequations}

We may then substitute \eqref{eq:left_end_points} and
\eqref{eq:right_end_points} into their respective equations from
\eqref{eq:rearranged_approx_sys} so that:
\begin{subequations} \label{eq:rearranged_approx_sys_endpoints}
\begin{align}
    \left(
        2 + 2r - k + k U_1^m + \frac{a k V_1^m}{1 + \lambda U_1^m}
    \right)
    U_{1}^{m+1} - 2r U_{2}^{m+1} &=
    \left(
        2 - 2r + k - k U_1^m - \frac{a k V_1^m}{1 + \lambda U_1^m}
    \right)
    U_{1}^{m} + 2r U_{2}^{m}
    \\
    \left(
        2 + 2s + \frac{k}{ab} - \frac{a k U_1^m}{b ( 1 + \lambda U_1^m )}
    \right)
    V_{1}^{m+1} - 2s V_{2}^{m+1} &=
    \left(
        2 - 2s - \frac{k}{ab} + \frac{a k U_1^m}{b ( 1 + \lambda U_1^m )}
    \right)
    V_{1}^{m} + 2s V_{2}^{m}
    \\
    \left(
        2 + 2r - k + k U_N^m + \frac{a k V_N^m}{1 + \lambda U_N^m}
    \right)
    U_{N}^{m+1} - 2r U_{N-1}^{m+1} &=
    \left(
        2 - 2r + k - k U_N^m - \frac{a k V_N^m}{1 + \lambda U_N^m}
    \right)
    U_{N}^{m} + 2r U_{N-1}^{m}
    \\
    \left(
        2 + 2s + \frac{k}{ab} - \frac{a k U_N^m}{b ( 1 + \lambda U_N^m )}
    \right)
    V_{N}^{m+1} - 2s V_{N-1}^{m+1} &=
    \left(
        2 - 2s - \frac{k}{ab} + \frac{a k U_N^m}{b ( 1 + \lambda U_N^m )}
    \right)
    V_{N}^{m} + 2s V_{N-1}^{m}
\end{align}
\end{subequations}

rewritten into the following matrix equations where:
\begin{subequations}
\begin{align*}
    L_u &= 2 + 2r - k + k U_n^m + \frac{a k V_n^m}{1 + \lambda U_n^m} \\
    R_u &= 2 - 2r + k - k U_n^m - \frac{a k V_n^m}{1 + \lambda U_n^m} \\
    L_v &= 2 + 2s + \frac{k}{ab} - \frac{a k U_n^m}{b ( 1 + \lambda U_n^m )} \\
    R_v &= 2 - 2s - \frac{k}{ab} + \frac{a k U_n^m}{b ( 1 + \lambda U_n^m )}
\end{align*}
\end{subequations}

\begin{align*}
\begin{bmatrix}
    L_u    & -2r    & \dots  & \dots  & 0 \\
    -r     & L_u    & -r     & \ddots & \vdots \\
    0      & \ddots & L_u    & \ddots & \vdots \\
    \vdots & \ddots & \ddots & \ddots & -r   \\
    0      & \dots  & \dots  & -2r    & L_u
\end{bmatrix}
\begin{bmatrix}
    U_1^{m+1}     \\
    U_2^{m+1}     \\
    U_3^{m+1}     \\
    \vdots        \\
    U_n^{m+1}
\end{bmatrix}
&=
\begin{bmatrix}
    R_u    & 2r     & \dots  & \dots  & 0      \\
    r      & R_u    & r      & \ddots & \vdots \\
    0      & \ddots & R_u    & \ddots & \vdots \\
    \vdots & \ddots & \ddots & \ddots & r      \\
    0      & \dots  & \dots  & 2r     & R_u
\end{bmatrix}
\begin{bmatrix}
    U_1^{m} \\
    U_2^{m} \\
    U_3^{m} \\
    \vdots  \\
    U_N^{m}
\end{bmatrix} \\[10pt]
\begin{bmatrix}
    L_v   & -2s     & \dots  & \dots  & 0       \\
    -s     & L_v    & -s     & \ddots & \vdots  \\
    0      & \ddots & L_v    & \ddots & \vdots  \\
    \vdots & \ddots & \ddots & \ddots & -s      \\
    0      & \dots  & \dots  & -2s    & L_v
\end{bmatrix}
\begin{bmatrix}
    V_1^{m+1}     \\
    V_2^{m+1}     \\
    V_3^{j+1}     \\
    \vdots        \\
    V_n^{m+1}
\end{bmatrix}
&=
\begin{bmatrix}
    R_v    & 2s     & \dots  & \dots  & 0 \\
    s      & R_v    & s      & \dots  & 0 \\
    0      & \ddots & R_v    & \ddots & \vdots \\
    \vdots & \ddots & \ddots & \ddots & s   \\
    0      & \dots  & \dots  & 2s     & R_v
\end{bmatrix}
\begin{bmatrix}
    V_1^{m}     \\
    V_2^{m}     \\
    V_3^{m}     \\
    \vdots      \\
    V_n^{m}
\end{bmatrix}
\end{align*}
